theories/Context.v
@@ -159,7 +159,7 @@ Fixpoint search σ E: list span :=
   end%list %map.
 
 Theorem typecheck_sound:
-  ∀ Δ {E Δ' t}, typecheck Δ E = Some (Δ', t) → JE Δ' E t.
+  ∀ Δ {E Δ' t}, typecheck Δ E = Some (Δ', t) → JE (l_with Δ' E) t.
 Proof using.
   intros Δ E.
   functional induction (typecheck Δ E).
@@ -607,10 +607,10 @@ Qed.
 
 Lemma subst_preserve:
   ∀ {Δ' E' t},
-    JE Δ' E' t →
+    JE (l_with Δ' E') t →
     ∀ {X E Δ t'},
-      JE (Map.merge (Map.one X t) Δ) E t' →
-      JE (Map.merge Δ' Δ) (subst_context E' X E) t'.
+      JE (l_with (Map.merge (Map.one X t) Δ) E) t' →
+      JE (l_with (Map.merge Δ' Δ) (subst_context E' X E)) t'.
 Proof using.
   intros Δ' E' t p X.
   intros E.
@@ -681,7 +681,7 @@ Proof.
     auto.
 Qed.
 
-Definition oftype Δ t := { E | JE Δ E t }.
+Definition oftype Δ t := { E | JE (l_with Δ E) t }.
 
 Definition equiv {Δ t}: Relation_Definitions.relation (oftype Δ t) :=
   λ a b,
